always use `addrFromKPPtr` for kernel addresses
This verifies a C kernel patch (seL4/seL4#409) which consolidates
translation between virtual and physical addresses, and makes it
consistent across architectures. In particular, we always use
`addrFromKPPtr`, even on architectures that don't use a distinct region
to map the kernel ELF. This will facilitate future improvements which
move the ELF mapping into a distinct virtual address region.

Signed-off-by: Matthew Brecknell <Matthew.Brecknell@data61.csiro.au>

spec/haskell/src/SEL4/Kernel/VSpace/ARM.lhs
@@ -937,7 +937,7 @@ If the current thread has no page directory, or if it has an invalid ASID, the h
 #else
 >             globalPD <- gets (armKSGlobalPD . ksArchState)
 #endif
->             doMachineOp $ setCurrentPD $ addrFromPPtr globalPD)
+>             doMachineOp $ setCurrentPD $ addrFromKPPtr globalPD)
 
 When cleaning the cache by user virtual address on ARM11, the active address space must be the one that contains the mappings being cleaned. The following function is used to temporarily switch to a given page directory and ASID, in order to clean the cache. It returns "True" if the address space was not the same as the current one, in which case the caller must switch back to the current address space once the cache is clean.
 
